wip

HumanEvalLean/HumanEval106.lean
@@ -1,3 +1,12 @@
+module
+
+import Std.Tactic.Do
+-- Sadly, it's apparently impossible to easily prove the size of a
+-- `Nat` range without unfolding internal stuff.
+import all Init.Data.Iterators.Consumers.Loop
+
+open Std.Do
+
 def f (n : Nat) : List Nat := Id.run do
   let mut ret : List Nat := []
   for i in 1...=n do
@@ -22,9 +31,160 @@ example : f 3 = [1, 2, 6] := by native_decide
 
 /-!
 ## Verification
-
-TODO
 -/
+
+def factorial : Nat → Nat
+  | 0 => 1
+  | n + 1 => factorial n * (n + 1)
+
+example : factorial 1 = 1 := by decide
+example : factorial 3 = 6 := by decide
+
+@[simp]
+theorem Std.PRange.length_toList_eq_size [UpwardEnumerable α] [LawfulUpwardEnumerable α]
+    [SupportsLowerBound sl α] [SupportsUpperBound su α] [BoundedUpwardEnumerable sl α]
+    [HasFiniteRanges su α] [RangeSize su α] [LawfulRangeSize su α]
+    {r : PRange ⟨sl, su⟩ α} :
+    r.toList.length = r.size := by
+  simp [PRange.toList, PRange.size]
+
+@[simp]
+theorem Nat.size_Rco {a b : Nat} :
+    (a...b).size = b - a := by
+  simp [Std.PRange.size, Std.Iterators.Iter.size, Std.Iterators.IteratorSize.size,
+    Std.PRange.Internal.iter, Std.Iterators.Iter.toIterM, Std.PRange.RangeSize.size]
+
+@[simp]
+theorem Nat.size_Rcc {a b : Nat} :
+    (a...=b).size = b + 1- a := by
+  simp [Std.PRange.size, Std.Iterators.Iter.size, Std.Iterators.IteratorSize.size,
+    Std.PRange.Internal.iter, Std.Iterators.Iter.toIterM, Std.PRange.RangeSize.size]
+
+theorem Std.PRange.getElem?_Rcx_eq [LE α] [UpwardEnumerable α] [LawfulUpwardEnumerable α]
+    [SupportsUpperBound su α]
+    [LawfulUpwardEnumerableLE α] [HasFiniteRanges su α]
+    {r : PRange ⟨.closed, su⟩ α} {i} :
+    r.toList[i]? = (UpwardEnumerable.succMany? i r.lower).filter (SupportsUpperBound.IsSatisfied r.upper) := by
+  sorry
+
+theorem Std.PRange.succMany?_isSome_of_lt_length_toList [LE α] [UpwardEnumerable α]
+    [LawfulUpwardEnumerable α] [SupportsUpperBound su α]
+    [LawfulUpwardEnumerableLE α] [HasFiniteRanges su α]
+    {r : PRange ⟨.closed, su⟩ α} {i} (h : i < r.toList.length) :
+    (UpwardEnumerable.succMany? i r.lower).isSome := by
+  sorry
+
+theorem Std.PRange.getElem_Rcx_eq [LE α] [UpwardEnumerable α] [LawfulUpwardEnumerable α]
+    [SupportsUpperBound su α]
+    [LawfulUpwardEnumerableLE α] [HasFiniteRanges su α]
+    {r : PRange ⟨.closed, su⟩ α} {i h} :
+    r.toList[i]'h = (UpwardEnumerable.succMany? i r.lower).get
+        (succMany?_isSome_of_lt_length_toList h) := by
+  simp [List.getElem_eq_getElem?_get, getElem?_Rcx_eq]
+
+theorem length_f {n : Nat} :
+    (f n).length = n := by
+  generalize hwp : f n = w
+  apply Std.Do.Id.of_wp_run_eq hwp
+  mvcgen
+  all_goals try infer_instance
+  case inv1 =>
+    exact ⇓⟨cur, xs⟩ => ⌜xs.length = cur.prefix.length⌝
+  case inv2 =>
+    -- factorial loop
+    exact ⇓⟨cur, xs⟩ => ⌜True⌝
+  case inv3 =>
+    -- sum loop
+    exact ⇓⟨cur, xs⟩ => ⌜True⌝
+  all_goals simp_all -- relies on `Nat.size_Rcc`
+
+abbrev SVal' (σs : List (Type u)) (α : Type u) : Type u := match σs with
+  | [] => α
+  | σ :: σs => σ → SVal σs α
+
+abbrev SPred' (σs : List (Type u)) : Type u := SVal σs (ULift Prop)
+
+def pure {σs : List (Type u)} (P : Prop) : SPred' σs := match σs with
+  | [] => ULift.up P
+  | _ :: _ => fun _ => pure P
+
+-- open Std PRange in
+-- @[spec]
+-- theorem Spec.forIn'_prange {α β : Type u}
+--     [Monad m] [WPMonad m ps]
+--     [UpwardEnumerable α]
+--     [SupportsUpperBound su α] [SupportsLowerBound sl α] [HasFiniteRanges su α]
+--     [BoundedUpwardEnumerable sl α] [LawfulUpwardEnumerable α]
+--     [LawfulUpwardEnumerableLowerBound sl α] [LawfulUpwardEnumerableUpperBound su α]
+--     {xs : PRange ⟨sl, su⟩ α} {init : β} {f : (a : α) → a ∈ xs → β → m (ForInStep β)}
+--     (inv : Invariant xs.toList β ps)
+--     (step : ∀ pref cur suff (h : xs.toList = pref ++ cur :: suff) b,
+--       Triple
+--         (f cur (by simp [←mem_toList_iff_mem, h]) b)
+--         (inv.1 (⟨pref, cur::suff, h.symm⟩, b))
+--         (fun r => match r with
+--           | .yield b' => inv.1 (⟨pref ++ [cur], suff, by simp [h]⟩, b')
+--           | .done b' => inv.1 (⟨xs.toList, [], by simp⟩, b'), inv.2)) :
+--     Triple (forIn' xs init f) (inv.1 (⟨[], xs.toList, rfl⟩, init)) (fun b => inv.1 (⟨xs.toList, [], by simp⟩, b), inv.2) := by
+--   simp only [forIn'_eq_forIn'_toList]
+--   apply Spec.forIn'_list inv step
+
+theorem f_eq_fac {n : Nat} {k : Nat} (hlt : k < n) (hmod : k % 2 = 1) :
+    (f n)[k]'(by grind [length_f]) = factorial (k + 1) := by
+  rw [List.getElem_eq_iff]
+  generalize hwp : f n = w
+  apply Std.Do.Id.of_wp_run_eq hwp
+  mvcgen
+  all_goals try infer_instance
+  case inv1 =>
+    exact ⇓⟨cur, xs⟩ => ⌜xs.length = cur.prefix.length ∧ ((_ : k < xs.length) → xs[xs.length - 1 - k] = factorial (k + 1))⌝
+  case inv2 =>
+    -- factorial loop
+    exact ⇓⟨cur, x⟩ => ⌜x = factorial cur.prefix.length⌝
+  case inv3 =>
+    -- sum loop => irrelevant
+    exact ⇓⟨cur, xs⟩ => ⌜True⌝
+  case vc3 =>
+    simp_all [factorial]
+    rename_i cur _ _ _ _ pref' cur' suff' h' _ _ _
+    have : cur' = (1...=cur).toList[pref'.length]'(by simp [h']) := by simp [h']
+    rw [this, Std.PRange.getElem_Rcx_eq]
+    simp only [Std.PRange.UpwardEnumerable.succMany?, Option.get_some]
+    grind
+  case vc4 => simp [factorial]
+  case vc5 =>
+    simp_all
+    intro h
+    rename_i pref cur suff _ _ _ _ _ _  h' _
+    have : cur = pref.length + 1 := sorry
+    obtain ⟨h', h''⟩ := h'
+    simp_all
+    rw [List.getElem_cons]
+    split
+    · simp_all
+      grind
+    · simp_all
+      refine Eq.trans ?_ (h'' ?_)
+      · grind
+      · grind only -- `grind` fails, see #10233
+  case vc7 => simp
+  case vc8 => simp
+  case vc9 =>
+    simp_all
+    intro h
+    rename_i pref cur suff _ _ _ _ _ h''
+    have : cur = pref.length + 1 := sorry
+    refine Eq.trans ?_ (h''.2 ?_)
+    simp_all
+    rw [List.getElem_cons]
+    · rw [dif_neg (by grind only)]
+      grind
+    · grind
+  case vc10 => simp
+  case vc11 =>
+    rename_i h
+    obtain ⟨h, h'⟩ := h
+    simp_all
 
 /-!
 ## Prompt
